refactor

Db/Query/Basic.lean
@@ -1,2 +1,113 @@
-inductive Query where
-  | all : Query
+import Std
+import Db.Utils.VarChar
+
+inductive DBType where
+  | bool : DBType
+  | int : DBType
+  | varchar (n : Nat) : DBType
+  deriving BEq, Repr, DecidableEq, Hashable
+
+protected def DBType.Value : DBType → Type
+  | .bool => Bool
+  | .varchar n => VarChar n
+  | .int => Int
+
+structure Column where
+  type : DBType
+  deriving BEq, Repr
+
+structure Table where
+  columns : Std.HashMap String Column
+
+structure Database where
+  tables : Std.HashMap String Table
+
+@[grind]
+def Database.HasTable (d : Database) (name : String) : Prop :=
+  name ∈ d.tables
+
+@[grind]
+def Table.HasColumn (t : Table) (name : String) : Prop :=
+  name ∈ t.columns
+
+structure Database.Ident (d : Database) where
+  tableName : String
+  columnName : String
+  hasTable : d.HasTable tableName := by grind
+  hasColumn : columnName ∈ d.tables[tableName].columns := by grind
+  deriving BEq, Hashable
+  -- btype_eq : d.tables[table].columns[column].btype = t := by grind
+
+attribute [grind] Database.Ident.hasTable Database.Ident.hasColumn
+
+def Database.Ident.table {d : Database} (i : d.Ident) : Table :=
+  d.tables[i.tableName]'(by grind)
+
+def Database.Ident.column {d : Database} (i : d.Ident) : Column :=
+  ((d.tables[i.tableName]'(by grind)).columns)[i.columnName]'(by grind)
+
+def Database.Ident.dbtype {d : Database} (i : d.Ident) : DBType :=
+  i.column.type
+
+def Table.idents {d : Database} (tname : String) (ht : d.HasTable tname) : Std.HashSet d.Ident :=
+  .ofList (d.tables[tname].columns.toList.pmap (P := fun a ↦ a ∈ d.tables[tname].columns.toList)
+    (fun c hmem ↦ ⟨tname, c.1, ht, by grind⟩) (by grind))
+
+instance (d : Database) (name : String) : Decidable (d.HasTable name) :=
+  inferInstanceAs <| Decidable (name ∈ d.tables)
+
+def Database.HasTable.get {d : Database} {name : String} (h : d.HasTable name) : Table :=
+  d.tables[name]
+
+def Database.HasColumn (d : Database) (table : String) (column : String) : Prop :=
+  ∃ (h : d.HasTable table), column ∈ d.tables[table].columns
+
+inductive DBExpr (d : Database) : DBType → Type 1 where
+  | true : DBExpr d .bool
+  | false : DBExpr d .bool
+  | and (e₁ e₂ : DBExpr d .bool) : DBExpr d .bool
+  | eq {t : DBType} (e₁ e₂ : DBExpr d t) : DBExpr d .bool
+
+inductive Database.Name (d : Database) where
+  | ident (i : d.Ident) : Name d
+  | computation (n : String) (t : DBType) : Name d
+  deriving BEq, Hashable
+
+def Database.Name.dbtype {d : Database} : d.Name → DBType
+  | .ident i => i.dbtype
+  | .computation _ t => t
+
+def Table.names {d : Database} (tname : String) (ht : d.HasTable tname := by grind) :
+    Std.HashSet d.Name :=
+  .ofList (d.tables[tname].columns.toList.pmap (P := fun a ↦ a ∈ d.tables[tname].columns.toList)
+    (fun c hmem ↦ .ident ⟨tname, c.1, ht, by grind⟩) (by grind))
+
+-- TODO: add join operations
+/--
+A query on the database `d` indexed over the (unique) names of the outputs.
+-/
+inductive Query (d : Database) : Std.HashSet d.Name → Type 1 where
+  | all (table : String) (ht : d.HasTable table := by grind) : Query d (Table.names table ht)
+  | filter {s : Std.HashSet d.Name} (q : Query d s) (e : DBExpr d .bool) : Query d s
+
+def signature {d : Database} (s : Std.HashSet d.Name) : Std.HashMap d.Name DBType :=
+  s.inner.map (fun n _ ↦ n.dbtype)
+
+def authors : Table where
+  columns := .ofList
+    [⟨"id", ⟨.int⟩⟩,
+     ⟨"name", ⟨.varchar 100⟩⟩,
+     ⟨"modern", ⟨.bool⟩⟩]
+
+def books : Table where
+  columns := .ofList
+    [⟨"name", ⟨.varchar 100⟩⟩,
+     ⟨"author", ⟨.varchar 100⟩⟩]
+
+abbrev database : Database where
+  tables := .ofList
+    [⟨"author", authors⟩,
+     ⟨"book", books⟩]
+
+example : Query database (Table.names "author") :=
+  .filter (.all "author") .true
