Db/Backends/Sql.lean
@@ -1,0 +1,45 @@
+import Db.Interpretation.Basic
+
+namespace SQL
+
+inductive Expr where
+  | true
+  | false
+  | eq (e₁ e₂ : Expr)
+  | and (e₁ e₂ : Expr)
+  | var (s : String)
+  deriving Repr
+
+def Expr.fromExpr {d : Database} {t : DBType} : DBExpr d t → Expr
+  | .true => true
+  | .false => false
+  | .eq e₁ e₂ => eq (fromExpr e₁) (fromExpr e₂)
+  | .and e₁ e₂ => and (fromExpr e₁) (fromExpr e₂)
+
+inductive Selector where
+  | fields (es : List Expr)
+  | all
+  deriving Repr
+
+structure Select where
+  selector : Selector
+  fromTable : String
+  condition : Expr
+  deriving Repr
+
+def Select.fromQuery {d : Database} {names : Std.HashSet d.Name} : Query d names → Select
+  | .all table ht => { selector := .all, fromTable := table, condition := .true}
+  | .filter q e =>
+    letI s := fromQuery q
+    { s with condition := .and s.condition (.fromExpr e) }
+
+def interpretation : Interpretation Select where
+  fromQuery _ := Select.fromQuery
+
+end SQL
+
+section Tests
+
+-- #eval SQL.Select.fromQuery (d := database) (.filter (.all "author") .true)
+
+end Tests
