Db/Interpretation/Basic.lean
@@ -1,0 +1,10 @@
+import Db.Query.Basic
+
+structure Interpretation (query : Type) where
+  fromQuery {d : Database} (names : Std.HashSet d.Name) (q : Query d names) : query
+
+/-- An interpretation monad on the database `d` provides lookup and modification operations. -/
+class DBMonad (d : Database) (m : Type → Type) where
+  /-- Lookup the given query on the database. -/
+  lookup {names : Std.HashSet d.Name} (q : Query d names) :
+    m (Std.DHashMap d.Name (fun d ↦ d.dbtype.Value))
